ChoiceTyping/theories/ResultWorldFreshForall.v
@@ -12,6 +12,27 @@ From CoreLang Require Import Instantiation InstantiationProps OperationalProps
 From ChoiceTyping Require Import ResultWorldBridge.
 From ChoiceType Require Import BasicStore LocallyNamelessProps.
 
+Lemma set_difference_pull_singleton (X Y : aset) x :
+  x ∈ X →
+  x ∉ Y →
+  X ∖ Y = (X ∖ ({[x]} ∪ Y)) ∪ {[x]}.
+Proof.
+  intros HxX HxY.
+  apply set_eq. intros z.
+  rewrite elem_of_difference, elem_of_union, elem_of_difference,
+    elem_of_union, !elem_of_singleton.
+  split.
+  - intros [HzX HzY].
+    destruct (decide (z = x)) as [->|Hzx].
+    + right. reflexivity.
+    + left. split; [exact HzX |].
+      intros [Hzx'|HzY']; [congruence | contradiction].
+  - intros [[HzX Hnot] | Hzx].
+    + split; [exact HzX |].
+      intros HzY. apply Hnot. right. exact HzY.
+    + subst z. split; [exact HxX | exact HxY].
+Qed.
+
 Lemma let_result_world_on_models_FExprResult :
   ∀ X e ν (n : WfWorld) Hfresh Hresult,
     fv_tm e ⊆ X →
@@ -19,9 +40,73 @@ Lemma let_result_world_on_models_FExprResult :
     ν ∉ X →
     X ⊆ world_dom (n : World) →
     world_store_closed_on X n →
-    let_result_world_on e ν n Hfresh Hresult ⊨ FExprResult e ν.
+    let_result_world_on e ν n Hfresh Hresult ⊨ FExprResultOn X e ν.
 Proof.
-Admitted.
+  intros X e ν n Hfresh Hresult Hfv Hlc HνX HXn Hclosed.
+  unfold res_models, FExprResultOn.
+  apply fib_vars_models_intro.
+  - unfold formula_scoped_in_world.
+    rewrite fib_vars_formula_fv. simpl.
+    unfold stale, stale_logic_qualifier. simpl.
+    rewrite dom_empty_L.
+    set_solver.
+  - set (nX := res_restrict n X).
+    assert (HfreshX : ν ∉ world_dom (nX : World)).
+    { subst nX. simpl. set_solver. }
+    assert (HresultX : ∀ σ, (nX : World) σ →
+      ∃ vx, subst_map (store_restrict σ (fv_tm e)) e →* tret vx).
+    {
+      subst nX. intros σ [σ0 [Hσ0 Hrestrict]].
+      destruct (Hresult σ0 Hσ0) as [vx Hsteps].
+      exists vx.
+      rewrite <- Hrestrict.
+      rewrite store_restrict_restrict.
+      replace (X ∩ fv_tm e) with (fv_tm e) by set_solver.
+      exact Hsteps.
+    }
+    set (result := res_restrict
+      (let_result_world_on e ν n Hfresh Hresult) (X ∪ {[ν]})).
+    assert (Hresult_eq :
+      result = let_result_world_on e ν nX HfreshX HresultX).
+    {
+      subst result nX.
+      apply let_result_world_on_restrict_input; eauto.
+    }
+    eapply fib_vars_obligation_intro
+      with (I := fun Fixed ρ w =>
+        result_world_slice_inv X ν result Fixed ρ w).
+    + eapply result_world_slice_inv_initial.
+      * subst result. simpl. set_solver.
+      * reflexivity.
+    + intros x Y ρ w HxX HxY Hinv.
+      eapply (result_world_slice_inv_disjoint
+        X ν result (X ∖ ({[x]} ∪ Y)) ρ w x); eauto.
+      set_solver.
+    + intros x Y ρ w HxX HxY Hinv Hdisj σx Hproj.
+      rewrite (set_difference_pull_singleton X Y x HxX HxY).
+      eapply (result_world_slice_inv_step
+        X ν result (X ∖ ({[x]} ∪ Y)) ρ w x σx Hproj); eauto.
+      set_solver.
+    + intros ρ w Hinv.
+      rewrite Hresult_eq in Hinv.
+      assert (HclosedX : world_store_closed_on X nX).
+      {
+        subst nX.
+        eapply world_store_closed_on_restrict.
+        - intros z Hz. exact Hz.
+        - exact Hclosed.
+      }
+      assert (HdomnX : world_dom (nX : World) = X).
+      {
+        subst nX. simpl.
+        apply set_eq. intros z. rewrite elem_of_intersection.
+        split.
+        - intros [_ HzX]. exact HzX.
+        - intros HzX. split; [apply HXn; exact HzX | exact HzX].
+      }
+      eapply (result_world_slice_inv_base X e ν nX HdomnX HfreshX HresultX
+        Hfv Hlc HclosedX); eauto.
+Qed.
 
 Lemma fresh_forall_expr_result_to_let_result_world_renamed
     X e D (body : atom → FormulaQ) (m : WfWorld) :
@@ -29,16 +114,17 @@ Lemma fresh_forall_expr_result_to_let_result_world_renamed
   lc_tm e →
   X ⊆ world_dom (m : World) →
   world_store_closed_on X m →
-  m ⊨ fresh_forall D (fun x => FImpl (FExprResult e x) (body x)) →
+  m ⊨ fresh_forall D (fun x => FImpl (FExprResultOn X e x) (body x)) →
   ∃ L : aset,
     world_dom (m : World) ∪ D ∪ X ∪ fv_tm e ⊆ L ∧
     ∀ y,
       y ∉ L →
       ∀ Hfresh Hresult,
-        (∀ n,
-          n ⊨ FExprResult e y →
+        (∀ (n : WfWorld),
+          world_dom (n : World) = world_dom (m : World) ∪ {[y]} →
+          n ⊨ FExprResultOn X e y →
           n ⊨ formula_rename_atom (fresh_for D) y
-                 (FExprResult e (fresh_for D))) →
+                 (FExprResultOn X e (fresh_for D))) →
         let_result_world_on e y m Hfresh Hresult ⊨
           formula_rename_atom (fresh_for D) y (body (fresh_for D)).
 Proof.
@@ -55,7 +141,7 @@ Proof.
   specialize (Himpl_fuel (let_result_world_on_restrict e y m Hfresh Hresult)).
   assert (Himpl :
     w ⊨ FImpl
-      (formula_rename_atom (fresh_for D) y (FExprResult e (fresh_for D)))
+      (formula_rename_atom (fresh_for D) y (FExprResultOn X e (fresh_for D)))
       (formula_rename_atom (fresh_for D) y (body (fresh_for D)))).
   {
     unfold res_models, res_models_with_store.
@@ -73,13 +159,14 @@ Proof.
   eapply res_models_impl_elim.
   - exact Himpl.
   - apply Hante.
-    subst w.
-    apply (let_result_world_on_models_FExprResult X).
-    + exact Hfv.
-    + exact Hlc.
-    + set_solver.
-    + simpl. set_solver.
-    + exact Hclosed.
+    + subst w. rewrite let_result_world_on_dom. reflexivity.
+    + subst w.
+      apply (let_result_world_on_models_FExprResult X).
+      * exact Hfv.
+      * exact Hlc.
+      * set_solver.
+      * simpl. set_solver.
+      * exact Hclosed.
 Qed.
 
 Lemma fresh_forall_expr_result_to_let_result_world
@@ -88,16 +175,17 @@ Lemma fresh_forall_expr_result_to_let_result_world
   lc_tm e →
   X ⊆ world_dom (m : World) →
   world_store_closed_on X m →
-  m ⊨ fresh_forall D (fun x => FImpl (FExprResult e x) (body x)) →
+  m ⊨ fresh_forall D (fun x => FImpl (FExprResultOn X e x) (body x)) →
   ∃ L : aset,
     world_dom (m : World) ∪ D ∪ X ∪ fv_tm e ⊆ L ∧
     ∀ y,
       y ∉ L →
       ∀ Hfresh Hresult,
-        (∀ n,
-          n ⊨ FExprResult e y →
+        (∀ (n : WfWorld),
+          world_dom (n : World) = world_dom (m : World) ∪ {[y]} →
+          n ⊨ FExprResultOn X e y →
           n ⊨ formula_rename_atom (fresh_for D) y
-                 (FExprResult e (fresh_for D))) →
+                 (FExprResultOn X e (fresh_for D))) →
         (∀ n,
           n ⊨ formula_rename_atom (fresh_for D) y (body (fresh_for D)) →
           n ⊨ body y) →
