ChoiceTyping/theories/Soundness.v
@@ -63,8 +63,6 @@ Proof.
   inversion Hbasicctx; subst; clear Hbasicctx.
   simpl in Hbind.
   unfold denot_ty_in_ctx_under, erase_ctx_under. simpl.
-  replace (dom (Σ ∪ {[x := erase_ty τ]})) with (dom Σ ∪ {[x]}).
-  2:{ rewrite dom_union_L, dom_singleton_L. reflexivity. }
   replace (Σ ∪ {[x := erase_ty τ]}) with (<[x := erase_ty τ]> Σ).
   - exact Hbind.
   - apply (map_eq (M := gmap atom)). intros z.
@@ -155,7 +153,7 @@ Lemma fundamental_const_case Σ c :
 Proof.
   intros m Hctx.
   unfold const_precise_ty, precise_ty, over_ty, under_ty.
-  unfold denot_ty_in_ctx_under, denot_ty_avoiding.
+  unfold denot_ty_in_ctx_under, denot_ty_on.
   simpl.
   eapply res_models_and_intro_from_models.
   - apply fundamental_const_over_case. exact Hctx.
@@ -330,15 +328,12 @@ Lemma semantic_total_let_rule (Φ : primop_ctx) Σ Γ τ1 τ2 e1 e2 (L : aset) :
 Proof.
   intros Hwf1 Hwf Hbody_wf IH1 IH2 m Hm.
   apply denot_ty_total_model_old.
-  eapply denot_tlet_total_at_world_split with (L := L).
+  eapply (denot_tlet_total_semantic Σ Γ τ1 τ2 e1 e2 L).
   - exact (proj2 Hwf1).
   - exact (proj2 Hwf).
+  - intros n Hn. eapply entails_total_to_total_model; eauto.
+  - intros x HxL n Hn. eapply entails_total_to_total_model; eauto.
   - exact Hm.
-  - eapply entails_total_to_total_model; eauto.
-  - exact (choice_typing_wf_basic_choice_ty_erased
-      Σ Γ (tlete e1 e2) τ2 Hwf).
-  - intros x HxL.
-    eapply entails_total_to_total_model; eauto.
 Qed.
 
 Lemma fundamental_total_let_case (Φ : primop_ctx) Σ Γ τ1 τ2 e1 e2 (L : aset) :
